Cleanup; and add powerpoint slides

parsplit.c
@@ -19,11 +19,11 @@ int thread_worker(void *arg) {
   }
 }
 
-struct task *make_tasks(unsigned n) {
-  struct task *tasks = (struct task *)malloc(n * sizeof (struct task));
+struct task *make_tasks(unsigned T) {
+  struct task *tasks = (struct task *)malloc(T * sizeof (struct task));
   unsigned i;
   if (!tasks) exit(1);
-  for (i=1; i<n; i++) {
+  for (i=1; i<T; i++) {
     struct task *t = tasks+i; /* need this workaround for VST issue #613 */
     t->go = makelock();
     t->done = makelock();
@@ -40,11 +40,11 @@ void initialize_task (struct task *tasks,
   tasks[i].closure=closure;
 }
 
-void do_tasks(struct task *tasks, unsigned n) {
+void do_tasks(struct task *tasks, unsigned T) {
   int i;
-  for (i=1; i<n; i++)
+  for (i=1; i<T; i++)
     release (tasks[i].go);
   tasks[0].f(tasks[0].closure);
-  for (i=1; i<n; i++)
+  for (i=1; i<T; i++)
     acquire (tasks[i].done);
 }
