verif_dotprod.v
@@ -9,31 +9,31 @@ Definition Vprog : varspecs. mk_varspecs prog. Defined.
 
 Open Scope logic.
 
-Definition delta n numt i := i*n/numt.
+Definition delta t T i := i*t/T.
 
-Lemma delta_range: forall n numt,
-   0 <= n -> 0 < numt ->
+Lemma delta_range: forall t T,
+   0 <= t -> 0 < T ->
   forall i,
-   0 <= i <= numt -> 0 <= delta n numt i <= n.
+   0 <= i <= T -> 0 <= delta t T i <= t.
 Proof.
 intros.
   intros. unfold delta.
   split.  apply Z_div_nonneg_nonneg.  nia. lia.
   rewrite Z.mul_comm.
-  apply Z.le_trans with (n * numt / numt).
+  apply Z.le_trans with (t * T / T).
   apply Z.div_le_mono; auto; try lia.
   apply Z.mul_le_mono_nonneg_l; lia.
   rewrite Z.div_mul; lia.
 Qed.
 
-Lemma delta_0: forall n numt, delta n numt 0 = 0.
+Lemma delta_0: forall t T, delta t T 0 = 0.
 Proof.
 intros. reflexivity.
 Qed.
 
-Lemma delta_numt: forall n numt,
-  0 <= n -> 0 < numt -> 
-  delta n numt numt = n.
+Lemma delta_T: forall t T,
+  0 <= t -> 0 < T -> 
+  delta t T T = t.
 Proof.
  intros. unfold delta.
  rewrite Z.mul_comm.
@@ -41,10 +41,10 @@ Proof.
  lia.
 Qed.
 
-Lemma delta_S: forall n,
- 0 <= n -> 
- forall numt i,
-  0 <= i < numt -> delta n numt i <= delta n numt (i+1).
+Lemma delta_S: forall t,
+ 0 <= t -> 
+ forall T i,
+  0 <= i < T -> delta t T i <= delta t T (i+1).
 Proof.
 intros.
 unfold delta.
@@ -63,18 +63,18 @@ Definition dotprod (v12: list float * list float) : float :=
   let y := map (uncurry Float.mul) (combine v1 v2) in
   sum y.
 
-Definition dotprod_f (numt: Z) (v12: list float * list float) : dtask_output_type :=
+Definition dotprod_f (T: Z) (v12: list float * list float) : dtask_output_type :=
  let '(v1,v2) := v12 in
  let y :=  map (uncurry Float.mul) (combine v1 v2) in
  let n := Zlength y in
-  sum (map (fun i => sum (sublist (delta n numt i) (delta n numt (i+1)) y)) (iota numt)).
+  sum (map (fun i => sum (sublist (delta n T i) (delta n T (i+1)) y)) (iota T)).
 
 Lemma dotprod_f_sanity :
- forall numt v12,
-  0 < numt ->
+ forall T v12,
+  0 < T ->
   (forall x y z, (Float.add (Float.add x y) z) = Float.add x (Float.add y z)) ->
   (forall x, Float.add Float.zero x = x) ->
-  dotprod_f numt v12 = dotprod v12.
+  dotprod_f T v12 = dotprod v12.
 Proof.
  intros ? ? H2 ? ?.
  (* Let's pretend we don't know that from assumption H0 one could actually prove False... *)
@@ -84,19 +84,19 @@ unfold dotprod_f, dotprod.
 destruct v12 as [v1 v2].
 simpl.
 set (n := Zlength _).
-set (d := delta n numt).
+set (d := delta n T).
 set (v := map (uncurry _) _) in *.
 clearbody v.
-transitivity (sum (sublist 0 (d numt) v)).
-2:{ rewrite sublist_same; auto; try lia. apply delta_numt; rep_lia. }
-rewrite <- (Z2Nat.id numt) by lia.
-assert (Z.of_nat (Z.to_nat numt) <= numt) by lia.
+transitivity (sum (sublist 0 (d T) v)).
+2:{ rewrite sublist_same; auto; try lia. apply delta_T; rep_lia. }
+rewrite <- (Z2Nat.id T) by lia.
+assert (Z.of_nat (Z.to_nat T) <= T) by lia.
 revert H2.
-induction (Z.to_nat numt); intro.
+induction (Z.to_nat T); intro.
 simpl. unfold d. rewrite delta_0. list_solve.
 rewrite inj_S. unfold Z.succ. rewrite iota_S by lia.
-pose proof delta_range n numt ltac:(rep_lia) ltac:(lia) (Z.of_nat n0) ltac:(rep_lia).
-pose proof delta_range n numt ltac:(rep_lia) ltac:(lia)  ((Z.of_nat n0)+1) ltac:(rep_lia).
+pose proof delta_range n T ltac:(rep_lia) ltac:(lia) (Z.of_nat n0) ltac:(rep_lia).
+pose proof delta_range n T ltac:(rep_lia) ltac:(lia)  ((Z.of_nat n0)+1) ltac:(rep_lia).
 fold d in H4, H5.
 rewrite (sublist_split 0 (d (Z.of_nat n0))).
 2: lia.
@@ -148,7 +148,7 @@ Definition answer_val (q: query) (v: val) :=
 
 Definition t_dtask := Tstruct _dotprod_task noattr.
 
-Definition dtask_pred (numt: Z) (input: dtask_input_type) (q: query) (p: val) :=
+Definition dtask_pred (T: Z) (input: dtask_input_type) (q: query) (p: val) :=
         let '(contents,(p1,p2)) := input in 
         let n := Zlength (fst contents) in 
         !! (n = Zlength (snd contents) /\ n <= Int.max_unsigned) &&
@@ -160,11 +160,11 @@ Definition dtask_pred (numt: Z) (input: dtask_input_type) (q: query) (p: val) :=
         data_at (q_share q) (tarray tdouble n) (map Vfloat (fst contents)) p1 *
         data_at (q_share q) (tarray tdouble n) (map Vfloat (snd contents)) p2.
 
-Arguments dtask_pred numt input q p : simpl never.
+Arguments dtask_pred T input q p : simpl never.
 
 Lemma dtask_pred_local_facts:
-  forall numt input q p,
-     dtask_pred numt input q p |-- !! isptr p.
+  forall T input q p,
+     dtask_pred T input q p |-- !! isptr p.
 Proof.
 intros.
 unfold dtask_pred.
@@ -175,8 +175,8 @@ Qed.
 #[export] Hint Resolve dtask_pred_local_facts : saturate_local.
 
 Lemma dtask_pred_valid_pointer:
-  forall numt input q p,
-   dtask_pred numt input q p |-- valid_pointer p.
+  forall T input q p,
+   dtask_pred T input q p |-- valid_pointer p.
 Proof.
 intros.
 unfold dtask_pred.
@@ -191,9 +191,9 @@ Qed.
 
 #[export] Hint Resolve dtask_pred_valid_pointer : valid_pointer.
 
-Lemma dtask_pred_input_eq: forall numt input1 input2  p,
-          dtask_pred numt input1 REMEMBER p * 
-          dtask_pred numt input2 ANSWER p 
+Lemma dtask_pred_input_eq: forall T input1 input2  p,
+          dtask_pred T input1 REMEMBER p * 
+          dtask_pred T input2 ANSWER p 
           |-- !! (input1 = input2).
 Proof.
 intros.
@@ -240,39 +240,39 @@ Qed.
 
 Definition dotprod_worker_spec :=
  DECLARE _dotprod_worker
- WITH numt: Z, clo : val, input: task_input_type
+ WITH T: Z, clo : val, input: task_input_type
  PRE [ tptr tvoid ]
-    PROP() PARAMS(clo) SEP (dtask_pred numt input ASK clo)
+    PROP() PARAMS(clo) SEP (dtask_pred T input ASK clo)
  POST [ tvoid ]
-    PROP() RETURN() SEP(dtask_pred numt input ANSWER clo).
+    PROP() RETURN() SEP(dtask_pred T input ANSWER clo).
 
-Definition fclo (gv: globals) (numt: Z) (dtp: val) : list (val*val) :=
+Definition fclo (gv: globals) (T: Z) (dtp: val) : list (val*val) :=
   map (fun i => (gv _dotprod_worker, 
-                         field_address0 (tarray t_dtask numt) (SUB i) dtp)) 
-        (iota numt).
+                         field_address0 (tarray t_dtask T) (SUB i) dtp)) 
+        (iota T).
 
-Definition tasking numt (gv: globals) :=
+Definition tasking T (gv: globals) :=
   EX tp:val, EX dtp: val,
-   !! (0 < numt < 10000) &&
-   data_at Ews tuint (vint numt) (gv _num_threads) *
+   !! (0 < T < 10000) &&
+   data_at Ews tuint (vint T) (gv _num_threads) *
    data_at Ews (tptr t_task) tp (gv _tasks) *
-   task_array dtask_package (fclo gv numt dtp) tp *
+   task_array dtask_package (fclo gv T dtp) tp *
    data_at Ews (tptr t_dtask) dtp (gv _dtasks) *
-   data_at_ Ews (tarray t_dtask numt) dtp.
+   data_at_ Ews (tarray t_dtask T) dtp.
 
 Definition dotprod_spec :=
   DECLARE _dotprod
-  WITH numt:Z, p1:val, p2: val, v1: list float, v2: list float, gv: globals
+  WITH T:Z, p1:val, p2: val, v1: list float, v2: list float, gv: globals
   PRE [ tptr tdouble, tptr tdouble, tuint ]
     PROP ( Zlength v1 = Zlength v2; Zlength v1 <= Int.max_unsigned)
     PARAMS ( p1; p2; Vint (Int.repr (Zlength v1))) GLOBALS(gv)
-    SEP (tasking numt gv;
+    SEP (tasking T gv;
            data_at Ews (tarray tdouble (Zlength v1)) (map Vfloat v1) p1;
            data_at Ews (tarray tdouble (Zlength v2)) (map Vfloat v2) p2)
   POST [ tdouble ]
     PROP()
-    RETURN (Vfloat (dotprod_f numt (v1,v2)))
-    SEP (tasking numt gv;
+    RETURN (Vfloat (dotprod_f T (v1,v2)))
+    SEP (tasking T gv;
            data_at Ews (tarray tdouble (Zlength v1)) (map Vfloat v1) p1;
            data_at Ews (tarray tdouble (Zlength v2)) (map Vfloat v2) p2).
 
@@ -308,11 +308,11 @@ Qed.
 
 #[export] Hint Resolve task_array_local_facts: saturate_local.
 
-Definition partial_dotprod_f (t numt: Z) (v12: list float * list float) : dtask_output_type :=
+Definition partial_dotprod_f (t T: Z) (v12: list float * list float) : dtask_output_type :=
  let '(v1,v2) := v12 in
  let y :=  map (uncurry Float.mul) (combine v1 v2) in
  let n := Zlength y in
-  sum (map (fun i => sum (sublist (delta n numt i) (delta n numt (i+1)) y)) (iota t)).
+  sum (map (fun i => sum (sublist (delta n T i) (delta n T (i+1)) y)) (iota t)).
 
 Lemma body_make_dotprod_tasks: semax_body Vprog Gprog f_make_dotprod_tasks make_dotprod_tasks_spec.
 Proof.
@@ -335,23 +335,23 @@ forward_if False. forward_call. contradiction. contradiction.
 forward_if True. contradiction. 
 forward.
 entailer!.
-rename t into numt.
+rename t into T.
 Intros. clear H0.
 deadvars!.
-forward_for_simple_bound numt
+forward_for_simple_bound T
  (EX t:Z, 
    PROP ( )
-   LOCAL (gvars gv; temp _T (vint numt))
+   LOCAL (gvars gv; temp _T (vint T))
    SEP (library.mem_mgr gv;
-   library.malloc_token Ews (tarray t_dtask numt) dtp;
-   data_at_ Ews (tarray t_dtask numt) dtp;
+   library.malloc_token Ews (tarray t_dtask T) dtp;
+   data_at_ Ews (tarray t_dtask T) dtp;
    task_array dtask_package (
         map (fun i => (gv _dotprod_worker, 
-                         field_address0 (tarray t_dtask numt) (SUB i) dtp)) 
-           (iota t)  ++ Zrepeat (Vundef, Vundef) (numt-t)) 
+                         field_address0 (tarray t_dtask T) (SUB i) dtp)) 
+           (iota t)  ++ Zrepeat (Vundef, Vundef) (T-t)) 
       tp;
    TT;
-   data_at Ews tuint (vint numt) (gv _num_threads);
+   data_at Ews tuint (vint T) (gv _num_threads);
    data_at Ews (tptr t_task) tp (gv _tasks);
    data_at Ews (tptr t_dtask) dtp (gv _dtasks)))%assert.
 -
@@ -363,7 +363,7 @@ forward.
 forward.
 set (fclo' := map _ _ ++ _).
 forward_call (tp, t, (gv _dotprod_worker), 
-                    field_address0 (tarray t_dtask numt) (SUB t) dtp,
+                    field_address0 (tarray t_dtask T) (SUB t) dtp,
                     fclo').
 entailer!.
 simpl.
@@ -390,113 +390,63 @@ unfold tasking.
 Exists tp dtp.
 rewrite prop_true_andp by lia.
 list_simplify.
-change (map _ _) with (fclo gv numt dtp).
+change (map _ _) with (fclo gv T dtp).
 cancel.
 Qed.
 
 Lemma field_at_SUB_t_DOT_result:
- forall t numt a dtp,
- 0 <= t < numt ->
- numt < 10000 ->
- field_compatible (tarray t_dtask numt) [] dtp ->
- field_at Ews (tarray t_dtask numt) [StructField _result; ArraySubsc t]
+ forall t T a dtp,
+ 0 <= t < T ->
+ T < 10000 ->
+ field_compatible (tarray t_dtask T) [] dtp ->
+ field_at Ews (tarray t_dtask T) [StructField _result; ArraySubsc t]
   (Vfloat a) dtp
  = field_at Ews t_dtask (DOT _result) (Vfloat a)
-      (field_address0 (tarray t_dtask numt) (SUB t) dtp).
-(* issue: VST-Floyd should have a lemma for composing paths like this. *)
+      (field_address0 (tarray t_dtask T) (SUB t) dtp).
 Proof.
-intros until 1. intro Hnumt. intros.
-rewrite !field_at_data_at.
-simpl.
-f_equal.
-assert (Ht: 20 * t < 20 * numt) by nia.
-rewrite !field_address_offset by auto with field_compatible.
-rewrite field_address0_offset by auto with field_compatible.
-rewrite field_address_offset.
-simpl.
-rewrite offset_offset_val.
-reflexivity.
-simpl.
-destruct H0 as [? [? [? [? ?]]]].
-destruct dtp; try contradiction.
-clear H0.
-split3; [ | | split3]; auto.
-red in H2 |- *.
-simpl.
-unfold sizeof in H2; simpl in H2.
-rewrite Z.max_r in H2 by lia.
-rewrite <- (Ptrofs.repr_unsigned i) in H2|-*.
-rewrite ptrofs_add_repr.
-rewrite Ptrofs.unsigned_repr in H2 by rep_lia.
-rewrite Ptrofs.unsigned_repr by rep_lia.
-lia.
-red in H3|-*.
-unfold offset_val.
-eapply align_compatible_rec_Tarray_inv in H3; [ | eassumption].
-simpl Ctypes.sizeof in H3.
-replace (Ptrofs.unsigned (Ptrofs.add i (Ptrofs.repr (0 + 20 * t))))
-  with (Ptrofs.unsigned i + 20 * t); auto.
-unfold Ptrofs.add.
-rewrite !Ptrofs.unsigned_repr; try nia.
-rep_lia.
-rewrite Ptrofs.unsigned_repr by rep_lia.
-red in H2.
-simpl sizeof in H2.
-rewrite Z.max_r in H2 by lia.
-rep_lia.
-split; auto. 
-simpl.
-right; right; right. left; auto.
+intros.
+replace (field_address0 (tarray t_dtask T) (SUB t) dtp) 
+ with (field_address (tarray t_dtask T) (SUB t) dtp)
+ by auto 50 with field_compatible.
+apply (field_at_app _ (tarray t_dtask T) (DOT _result) (SUB t)); auto.
 Qed.
 
 Lemma finish_dotprod:
- forall numt p1 p2 v1 v2 dtp gv,
+ forall T p1 p2 v1 v2 dtp gv,
   Zlength v1 = Zlength v2 ->
-  0 < numt < 10000 ->
-  let delt := delta (Zlength v1) numt in
+  0 < T < 10000 ->
+  let delt := delta (Zlength v1) T in
 let inp :=
   map
     (fun i : Z =>
      ((sublist (delt i) (delt (i + 1)) v1, sublist (delt i) (delt (i + 1)) v2),
       (field_address0 (tarray tdouble (Zlength v1)) (SUB delt i) p1,
        field_address0 (tarray tdouble (Zlength v1)) (SUB delt i) p2)))
- (iota numt) in
-field_compatible (tarray t_dtask numt) [] dtp ->
+ (iota T) in
+field_compatible (tarray t_dtask T) [] dtp ->
 field_compatible0 (tarray tdouble (Zlength v1)) [] p1 ->
 field_compatible0 (tarray tdouble (Zlength v1)) [] p2 ->
-pred_sepcon (ith_spectask dtask_package (fclo gv numt dtp) inp ANSWER)
-  (fun i : Z => 0 <= i < numt)
-|-- data_at_ Ews (tarray t_dtask numt) dtp
+pred_sepcon (ith_spectask dtask_package (fclo gv T dtp) inp ANSWER)
+  (fun i : Z => 0 <= i < T)
+|-- data_at_ Ews (tarray t_dtask T) dtp
       * data_at Ews (tarray tdouble (Zlength v1)) (map Vfloat v1) p1
       * data_at Ews (tarray tdouble (Zlength v1)) (map Vfloat v2) p2.
 Proof.
 intros.
-set (t:=numt).
+set (t:=T).
 unfold t at 1.
 replace (data_at Ews (tarray tdouble (Zlength v1)) (map Vfloat v1) p1)
-  with (data_at Ews (tarray tdouble (delt t)) (map Vfloat (sublist 0 (delt t) v1)) p1).
-2:{ unfold t. unfold delt.
-  rewrite delta_numt by rep_lia.
- f_equal. f_equal.
- apply sublist_same; auto.
-}
-
+  with (data_at Ews (tarray tdouble (delt t)) (map Vfloat (sublist 0 (delt t) v1)) p1)
+  by (unfold t, delt; rewrite delta_T, sublist_same by rep_lia; auto).
 replace (data_at Ews (tarray tdouble (Zlength v1)) (map Vfloat v2) p2)
-  with (data_at Ews (tarray tdouble (delt t)) (map Vfloat (sublist 0 (delt t) v2)) p2).
-2:{ unfold t. unfold delt.
- rewrite H.
-  rewrite delta_numt by rep_lia.
- f_equal. f_equal.
- apply sublist_same; auto.
-}
-assert (0 <= t <= numt) by lia.
+  with (data_at Ews (tarray tdouble (delt t)) (map Vfloat (sublist 0 (delt t) v2)) p2)
+  by (unfold t, delt; rewrite delta_T, sublist_same by rep_lia; auto).
+assert (0 <= t <= T) by lia.
 clearbody t.
 rewrite <- (Z2Nat.id t) in * by lia.
 induction (Z.to_nat t).
 -
-replace (fun i : Z => 0 <= i < Z.of_nat 0) with (fun i:Z => False)
-  by (extensionality j; apply prop_ext; split; intro; lia).
-rewrite pred_sepcon_False.
+rewrite pred_sepcon_False' by lia.
 simpl Z.of_nat.
 unfold delt; rewrite delta_0.
 apply derives_trans with (emp * emp * emp).
@@ -506,12 +456,11 @@ repeat apply sepcon_derives; apply data_at_zero_array;
 -
 rewrite inj_S. unfold Z.succ. 
 rewrite (pred_sepcon_isolate (Z.of_nat n) zeq) by lia.
-unfold ith_spectask.
-sep_apply func_ptr'_emp.
 replace (fun y : Z => 0 <= y < Z.of_nat n + 1 /\ y <> Z.of_nat n)
  with (fun i : Z => 0 <= i < Z.of_nat n)
   by (extensionality j; apply prop_ext; split; intro; lia).
-fold (ith_spectask  dtask_package (fclo gv numt dtp) inp ANSWER).
+unfold ith_spectask at 2.
+sep_apply func_ptr'_emp.
 sep_apply IHn; try lia.
 clear IHn.
 clear t.
@@ -524,13 +473,11 @@ unfold fclo.
 rewrite !Znth_map by (rewrite ?Zlength_iota; lia).
 simpl.
 Intros. clear H5 H6.
-pose proof delta_range n numt ltac:(rep_lia) ltac:(lia) (Z.of_nat t) ltac:(lia). fold delt in H5.
-pose proof delta_range n numt ltac:(rep_lia) ltac:(lia) (Z.of_nat t + 1) ltac:(lia). fold delt in H6.
-pose proof delta_S n ltac:(lia) numt (Z.of_nat t) ltac:(lia). fold delt in H7.
+pose proof delta_range n T ltac:(rep_lia) ltac:(lia) (Z.of_nat t) ltac:(lia). fold delt in H5.
+pose proof delta_range n T ltac:(rep_lia) ltac:(lia) (Z.of_nat t + 1) ltac:(lia). fold delt in H6.
+pose proof delta_S n ltac:(lia) T (Z.of_nat t) ltac:(lia). fold delt in H7.
 rewrite !Znth_iota by lia.
 rewrite !Zlength_sublist by lia.
-change (data_at_ ?sh ?t ?p) 
-  with (data_at sh t (default_val t) p).
 sep_apply (field_at_share_join Ers Ers2 Ews t_dtask (DOT _vec1)); auto with shares.
 sep_apply (field_at_share_join Ers Ers2 Ews t_dtask (DOT _vec2)); auto with shares.
 sep_apply (field_at_share_join Ers Ers2 Ews t_dtask (DOT _n)); auto with shares.
@@ -538,73 +485,34 @@ sep_apply (field_at_field_at_ Ews t_dtask (DOT _vec1)).
 sep_apply (field_at_field_at_ Ews t_dtask (DOT _vec2)).
 sep_apply (field_at_field_at_ Ews t_dtask (DOT _n)).
 sep_apply (field_at_field_at_ Ews t_dtask (DOT _result)).
-assert (
- field_at_ Ews t_dtask (DOT _vec1)
-                 (field_address0 (tarray t_dtask numt) (SUB Z.of_nat t) dtp)
-* field_at_ Ews t_dtask (DOT _vec2)
-            (field_address0 (tarray t_dtask numt) (SUB Z.of_nat t) dtp)
-* field_at_ Ews t_dtask (DOT _n)
-       (field_address0 (tarray t_dtask numt) (SUB Z.of_nat t) dtp)
-* field_at_ Ews t_dtask (DOT _result)
-  (field_address0 (tarray t_dtask numt) (SUB Z.of_nat t) dtp)
-|-- data_at_ Ews t_dtask 
-  (field_address0 (tarray t_dtask numt) (SUB Z.of_nat t) dtp)). {
- unfold_data_at (data_at_ _ _ _).
- simpl. cancel.
-}
-sep_apply H8; clear H8.
-change (data_at_ ?sh ?t ?p) 
-  with (data_at sh t (default_val t) p).
-sep_apply (data_at_singleton_array Ews t_dtask [default_val t_dtask] _ 
-          (field_address0 (tarray t_dtask numt) (SUB Z.of_nat t) dtp) (eq_refl _)).
-pose proof split2_data_at_Tarray_app 
-  (delt (Z.of_nat t)) (delt (Z.of_nat t + 1)) Ews.
-set (dta := default_val (tarray t_dtask (Z.of_nat t)) : list (reptype t_dtask)).
-set (dtb := [default_val t_dtask] : list (reptype t_dtask)).
-pose proof (split2_data_at_Tarray_app (Z.of_nat t) (Z.of_nat t+1) Ews
-                       t_dtask dta dtb dtp). 
-spec H9. { 
- subst dta. unfold default_val; simpl.
-  rewrite Zlength_Zrepeat by lia. auto.
-}
-spec H9. { 
- subst dtb. simpl. list_solve. 
-}
-pose proof (derives_refl' _ _ (eq_sym H9)).
-replace (field_address0 (tarray t_dtask (Z.of_nat t + 1)) (SUB Z.of_nat t) dtp)
- with (field_address0 (tarray t_dtask numt)  (SUB Z.of_nat t) dtp)
- in H10.
-2:{
-rewrite !field_address0_offset by auto with field_compatible.
-reflexivity.
-}
-replace (Z.of_nat t + 1 - Z.of_nat t) with 1 in H10 by lia.
-sep_apply H10.
-clear H9 H10.
-cancel.
-rewrite !(sublist_split 0 (delt (Z.of_nat t)) (delt (Z.of_nat t + 1))) by lia.
-rewrite !map_app.
-rewrite !(split2_data_at_Tarray_app (delt (Z.of_nat t)) (delt (Z.of_nat t + 1)) 
-    Ews tdouble) by list_solve.
-cancel.
-clear H8 dta dtb.
+rewrite (split2_data_at__Tarray_app (Z.of_nat  t) (Z.of_nat t + 1)) by lia.
+
+replace (Z.of_nat t + 1 - Z.of_nat t) with 1 by lia.
+replace  (field_address0 (tarray t_dtask (Z.of_nat t + 1)) (SUB Z.of_nat t) dtp)
+ with  (field_address0 (tarray t_dtask (Z.of_nat t)) (SUB Z.of_nat t) dtp)
+ by (auto with field_compatible).
 set (dt := delt (Z.of_nat t)) in *.
 set (dt1 := delt (Z.of_nat t + 1)) in *.
-clearbody dt. clearbody dt1. clear t H1 delt H4.
+
+sep_apply (data_at_share_join Ers Ers2 Ews (tarray tdouble (dt1-dt))); auto with shares.
+sep_apply (data_at_share_join Ers Ers2 Ews (tarray tdouble (dt1-dt))); auto with shares.
+cancel.
+rewrite data__at_singleton_array_eq.
+unfold_data_at (data_at_ _ _ _).
+repeat change (field_at ?sh ?t ?f _) with (field_at_ sh t f).
+repeat replace (field_address0 (tarray t_dtask (Z.of_nat t)) (SUB Z.of_nat t) dtp)
+ with (field_address0 (tarray t_dtask T) (SUB Z.of_nat t) dtp)
+  by (auto with field_compatible).
+
+rewrite !(sublist_split 0 dt dt1) by lia.
+rewrite !map_app.
+rewrite !(split2_data_at_Tarray_app dt dt1) by list_solve.
 replace (field_address0 (tarray tdouble dt1) (SUB dt) p1)
- with  (field_address0 (tarray tdouble n) (SUB dt) p1).
-2:{
-rewrite !field_address0_offset by auto with field_compatible.
-reflexivity.
-}
+  with (field_address0 (tarray tdouble n) (SUB dt) p1)
+  by (auto with field_compatible).
 replace (field_address0 (tarray tdouble dt1) (SUB dt) p2)
- with  (field_address0 (tarray tdouble n) (SUB dt) p2).
-2:{
-rewrite !field_address0_offset by auto with field_compatible.
-reflexivity.
-}
-sep_apply (data_at_share_join Ers Ers2 Ews (tarray tdouble (dt1-dt))); auto with shares.
-sep_apply (data_at_share_join Ers Ers2 Ews (tarray tdouble (dt1-dt))); auto with shares.
+  with (field_address0 (tarray tdouble n) (SUB dt) p2)
+  by (auto with field_compatible).
 cancel.
 Qed.
 
@@ -612,7 +520,7 @@ Lemma body_dotprod: semax_body Vprog Gprog f_dotprod dotprod_spec.
 Proof.
 start_function.
 unfold tasking. Intros tp dtp.
-assert_PROP (field_compatible (tarray t_dtask numt) nil dtp) as Hdtp by entailer!.
+assert_PROP (field_compatible (tarray t_dtask T) nil dtp) as Hdtp by entailer!.
 rewrite <- H.
 set (n := Zlength v1) in *.
 assert (Hn: 0 <= n) by apply Zlength_nonneg.
@@ -620,13 +528,13 @@ forward.
 forward.
 
 assert_PROP (field_compatible0 (tarray tdouble n) nil p1 /\
-                    field_compatible0 (tarray tdouble n) nil p2) by  entailer!.
+                    field_compatible0 (tarray tdouble n) nil p2) as H2 by  entailer!.
 destruct H2.
-pose proof delta_range n numt.
-set (delt := delta n numt) in *.
+pose proof delta_range n T.
+set (delt := delta n T) in *.
 assert (Hforce:  
          forall t p, 
-          0 <= t <= numt -> 
+          0 <= t <= T -> 
           field_compatible0 (tarray tdouble n) [] p ->
         force_val
            (sem_add_ptr_int tdouble Unsigned p (vint (delt t))) 
@@ -641,29 +549,29 @@ assert (Hforce:
   
 freeze FR1 := - (data_at Ews (tptr t_task) tp (gv _tasks))
                 (data_at Ews (tptr t_dtask) dtp (gv _dtasks))
-               (data_at_ Ews  (tarray t_dtask numt) dtp).
+               (data_at_ Ews  (tarray t_dtask T) dtp).
 pose (nthtask i := (field_address0 (tarray tdouble n) (SUB (delt i)) p1,
                             (field_address0 (tarray tdouble n) (SUB (delt i)) p2,
                              (Vint (Int.repr (delt (i+1) - delt i)), Vundef)))).
-forward_for_simple_bound numt 
+forward_for_simple_bound T 
    (EX t:Z,   
     PROP ()
-    LOCAL (temp _delta (vint (delt t)); temp _T (vint numt);
+    LOCAL (temp _delta (vint (delt t)); temp _T (vint T);
                 gvars gv; temp _vec1 p1; temp _vec2 p2; 
                 temp _n (vint n))
    SEP (FRZL FR1;
           data_at Ews (tptr t_task) tp (gv _tasks);
           data_at Ews (tptr t_dtask) dtp (gv _dtasks);
-          data_at Ews (tarray t_dtask numt) 
+          data_at Ews (tarray t_dtask T) 
              (map nthtask (iota t)
-                     ++ Zrepeat (default_val t_dtask) (numt-t))
+                     ++ Zrepeat (default_val t_dtask) (T-t))
              dtp ))%assert.
 -
 entailer!. apply derives_refl.
 -
 rename i into t.
 pose proof (H4 ltac:(lia) ltac:(lia) t).
-replace (numt-t) with (1+(numt-(t+1))) by lia.
+replace (T-t) with (1+(T-(t+1))) by lia.
 rewrite <- Zrepeat_app by lia.
 change (Zrepeat (default_val t_dtask) 1) with [ (Vundef,(Vundef,(Vundef,Vundef))) ].
 forward.
@@ -680,7 +588,7 @@ list_simplify.
 
 forward.
 forward.
-rewrite Hforce by (auto; lia).
+rewrite Hforce by (auto; lia). clear Hforce.
 list_simplify.
 rewrite upd_Znth_app2, upd_Znth_app1 by Zlength_solve. 
 rewrite Zlength_map, Zlength_iota, Z.sub_diag by lia.
@@ -692,9 +600,9 @@ list_simplify.
 forward.
 entailer!.
 rewrite Int.unsigned_repr in H16 by rep_lia.
-assert (numt = 0); [ | lia].
+assert (T = 0); [ | lia].
 clear - H16 H1.
-rewrite <- (Int64.unsigned_repr numt) by rep_lia.
+rewrite <- (Int64.unsigned_repr T) by rep_lia.
 rewrite H16. reflexivity.
 rewrite add_repr.
 rewrite !Int.unsigned_repr by rep_lia.
@@ -702,7 +610,7 @@ rewrite mul64_repr.
 
 rewrite divu64_repr; [ | | rep_lia].
 2:{ clear - H5 H0 Hn H1.
-  assert (numt * Int.max_unsigned <= Int64.max_unsigned) by rep_lia.
+  assert (T * Int.max_unsigned <= Int64.max_unsigned) by rep_lia.
   split; try lia.
   eapply Z.le_trans; [ | apply H].
   apply Z.mul_le_mono_nonneg; lia.
@@ -718,8 +626,8 @@ apply Z.div_le_upper_bound. lia.
 
 forward.
 forward.
-change (let (q, _) := Z.div_eucl ((t + 1) * n) numt in q) with ((t+1)*n/numt).
-change ((t+1)*n/numt) with (delt (t+1)).
+fold ((t+1)*n/T).
+change ((t+1)*n/T) with (delt (t+1)).
 list_simplify.
 rewrite upd_Znth_app2, upd_Znth_app1 by Zlength_solve. 
 rewrite Zlength_map, Zlength_iota, Z.sub_diag by lia.
@@ -731,18 +639,16 @@ list_simplify.
 forward.
 
 entailer!.
-apply  derives_refl'.
-f_equal.
 rewrite iota_S by lia.
 rewrite map_app.
 rewrite <- !app_assoc.
-reflexivity.
+apply  derives_refl.
 
 -
 list_simplify.
 thaw FR1.
-make_func_ptr _dotprod_worker. 
- change (func_ptr' _) with (func_ptr' (snd dotprod_worker_spec)).
+make_func_ptr _dotprod_worker.
+change (func_ptr' _) with (func_ptr' (snd dotprod_worker_spec)).
 assert_PROP (isptr tp) by entailer!.
 forward.
 pose (inp := (map (fun i => 
@@ -750,46 +656,37 @@ pose (inp := (map (fun i =>
                                 sublist (delt i) (delt(i+1)) v2),
                                (field_address0 (tarray tdouble n) (SUB delt i) p1,
                                 field_address0 (tarray tdouble n) (SUB delt i) p2)))
-                          (iota numt))).
-forward_call (fclo gv numt dtp ,inp,tp).
-apply prop_right.
-simpl. f_equal. f_equal. f_equal. unfold fclo. f_equal. autorewrite with sublist. rewrite Zlength_iota. auto.
-lia.
+                          (iota T))).
+forward_call (fclo gv T dtp ,inp,tp).
+  apply prop_right; unfold fclo; list_solve.
+ 2: unfold fclo; list_solve.
+{
+ subst Frame.
+ instantiate (1 := [data_at Ews tuint (vint T) (gv _num_threads);
+                   data_at Ews (tptr t_task) tp (gv _tasks);
+                   data_at Ews (tptr t_dtask) dtp (gv _dtasks)]).
+ simpl fold_right_sepcon.
+ cancel.
 
-assert (
-  func_ptr' (snd dotprod_worker_spec) (gv _dotprod_worker)
-  * data_at Ews (tarray tdouble n) (map Vfloat v1) p1
-  * data_at Ews (tarray tdouble n) (map Vfloat v2) p2
-  * data_at Ews (tarray t_dtask numt) (map nthtask (iota numt)) dtp
- |-- spectasks_list dtask_package (fclo gv numt dtp) inp ASK);
- [ | sep_apply H8; cancel]. {
  unfold spectasks_list.
  rewrite pred_sepcon_eq.
- Exists (iota numt).
- rewrite prop_true_andp.
- 2:{ split. intros.
-   unfold fclo. rewrite Zlength_map, Zlength_iota by lia.
-
- apply in_iota.
- apply NoDup_iota.
- }
-pose proof delta_numt n numt ltac:(lia) ltac:(lia). fold delt in H8.
- assert (data_at Ews (tarray tdouble n) (map Vfloat v1) p1
-        |-- data_at Ews (tarray tdouble (delt numt)) (map Vfloat (sublist 0 (delt numt) v1)) p1).
-   clear - H8. rewrite sublist_same by auto. rewrite H8. cancel.
- sep_apply H9. clear H9.
- assert (data_at Ews (tarray tdouble n) (map Vfloat v2) p2
-        |-- data_at Ews (tarray tdouble (delt numt)) (map Vfloat (sublist 0 (delt numt) v2)) p2).
-   clear - H H8. rewrite H8.  rewrite sublist_same by auto. cancel.
- sep_apply H9. clear H9.
- assert_PROP (field_compatible (tarray t_dtask numt) nil dtp) by entailer!.
+ Exists (iota T).
+ rewrite prop_true_andp
+   by (split; [intros; unfold fclo; rewrite Zlength_map, Zlength_iota by lia; 
+               apply in_iota| apply NoDup_iota]).
+ pose proof delta_T n T ltac:(lia) ltac:(lia). fold delt in H8.
+ rewrite <- (sublist_same _  (delt T) (map Vfloat v1) (eq_refl _))
+  by (   unfold fclo; rewrite Zlength_map, ?Zlength_iota; lia).
+ rewrite <- (sublist_same _  (delt T) (map Vfloat v2) (eq_refl _))
+  by (   unfold fclo; rewrite Zlength_map, ?Zlength_iota; lia).
+ rewrite <- H8.
+ assert_PROP (field_compatible (tarray t_dtask T) nil dtp) by entailer!.
  clear - H1 H H0 H2 H3 H9.
  set (fclo1 := fclo _ _ _).
- rewrite <- (Z2Nat.id numt) by lia.
- assert (Z.of_nat (Z.to_nat numt) <= numt) by lia.
+ rewrite <- (Z2Nat.id T) by lia.
+ assert (Z.of_nat (Z.to_nat T) <= T) by lia.
  revert H4.
- forget (Z.to_nat numt) as t.
- rewrite !map_sublist.
+ forget (Z.to_nat T) as t.
  induction t; intros.
  simpl. change (delt  0) with 0.
  sep_apply data_at_zero_array_inv.
@@ -797,10 +694,10 @@ pose proof delta_numt n numt ltac:(lia) ltac:(lia). fold delt in H8.
  sep_apply data_at_zero_array_inv.
  sep_apply func_ptr'_emp.
  cancel.
- pose proof delta_range n numt ltac:(rep_lia) ltac:(lia) (Z.of_nat t) ltac:(lia). fold delt in H5.
- pose proof delta_range n numt ltac:(rep_lia) ltac:(lia) (Z.of_nat t + 1) ltac:(lia). fold delt in H6.
+ pose proof delta_range n T ltac:(rep_lia) ltac:(lia) (Z.of_nat t) ltac:(lia). fold delt in H5.
+ pose proof delta_range n T ltac:(rep_lia) ltac:(lia) (Z.of_nat t + 1) ltac:(lia). fold delt in H6.
  rename H6 into H5'.
- pose proof delta_S n ltac:(lia) numt (Z.of_nat t) ltac:(lia). fold delt in H6.
+ pose proof delta_S n ltac:(lia) T (Z.of_nat t) ltac:(lia). fold delt in H6.
  rewrite inj_S. unfold Z.succ. rewrite iota_S by lia.
  rewrite iter_sepcon_app.
  rewrite !(sublist_split 0 (delt (Z.of_nat t)) (delt (Z.of_nat t + 1)))
@@ -817,24 +714,18 @@ change (@app (val * (val * (val * val)))) with (@app (reptype t_dtask)).
  apply derives_refl.
  unfold iter_sepcon.
  unfold ith_spectask.
- replace (fst (Znth (Z.of_nat t) fclo1)) with (gv _dotprod_worker).
+ replace (fst (Znth (Z.of_nat t) fclo1)) with (gv _dotprod_worker)
+   by (unfold fclo1, fclo; list_solve).
  change (snd dotprod_worker_spec)
    with (task_f_spec dtask_package).
  cancel.
- 2:{ subst fclo1.
-      unfold fclo. rewrite Znth_map. reflexivity.
-      rewrite Zlength_iota; lia.
-    }
  simpl task_pred. unfold dtask_pred.
  subst inp.
     rewrite !Znth_map by (rewrite Zlength_iota; lia).
  simpl.
- rewrite prop_true_andp.
-2:{ rewrite ?Znth_iota by lia.
- rewrite !Zlength_sublist by lia. lia.
-}
+ rewrite prop_true_andp by (rewrite ?Znth_iota by lia;  list_solve).
  subst fclo1. unfold fclo.
-    rewrite !Znth_map by (rewrite Zlength_iota; lia).
+ rewrite !Znth_map by (rewrite Zlength_iota; lia).
   simpl fst. simpl snd.
   rewrite !Zlength_sublist by (rewrite Znth_iota by lia; lia).
   replace (Z.of_nat t + 1 - Z.of_nat t) with 1 by lia.
@@ -842,54 +733,42 @@ change (@app (val * (val * (val * val)))) with (@app (reptype t_dtask)).
   unfold nthtask.
   unfold_data_at (data_at _ t_dtask _ _).
   rewrite Znth_iota by lia.
-assert (field_address0 (tarray t_dtask  (Z.of_nat t + 1)) (SUB Z.of_nat t) dtp
-         =  field_address0 (tarray t_dtask numt) (SUB Z.of_nat t) dtp). {
-  rewrite  !field_address0_offset by auto with field_compatible.
-  reflexivity. 
-}
  rewrite prop_true_andp by (split; lia).
  set (k := delt _ - delt _).
-
- rewrite !H7. clear H7.
+ replace (field_address0 (tarray t_dtask  (Z.of_nat t + 1)) (SUB Z.of_nat t) dtp)
+        with (field_address0 (tarray t_dtask T) (SUB Z.of_nat t) dtp)
+  by auto with field_compatible.
  rewrite !sublist_map.
-rewrite <-  (field_at_share_join Ers Ers2 Ews t_dtask (DOT _vec1)); auto with shares.
-rewrite <- (field_at_share_join Ers Ers2 Ews t_dtask (DOT _vec2)); auto with shares.
-rewrite <- (field_at_share_join Ers Ers2 Ews t_dtask (DOT _n)); auto with shares.
+ rewrite <-  (field_at_share_join Ers Ers2 Ews t_dtask (DOT _vec1)); auto with shares.
+ rewrite <- (field_at_share_join Ers Ers2 Ews t_dtask (DOT _vec2)); auto with shares.
+ rewrite <- (field_at_share_join Ers Ers2 Ews t_dtask (DOT _n)); auto with shares.
  cancel.
- assert (field_address0 (tarray tdouble (delt (Z.of_nat t + 1))) (SUB delt (Z.of_nat t)) p1
-       = field_address0 (tarray tdouble n) (SUB delt (Z.of_nat t)) p1). {
-    rewrite  !field_address0_offset by auto with field_compatible.
-    reflexivity.
-}
- rewrite H7; clear H7.
- assert (field_address0 (tarray tdouble (delt (Z.of_nat t + 1))) (SUB delt (Z.of_nat t)) p2
-       = field_address0 (tarray tdouble n) (SUB delt (Z.of_nat t)) p2). {
-    rewrite  !field_address0_offset by auto with field_compatible.
-    reflexivity.
-}
- rewrite H7; clear H7.
-rewrite <- !(data_at_share_join Ers Ers2 Ews) by auto with shares.
+ replace (field_address0 (tarray tdouble (delt (Z.of_nat t + 1))) (SUB delt (Z.of_nat t)) p1)
+       with (field_address0 (tarray tdouble n) (SUB delt (Z.of_nat t)) p1)
+  by auto with field_compatible.
+replace (field_address0 (tarray tdouble (delt (Z.of_nat t + 1))) (SUB delt (Z.of_nat t)) p2)
+    with (field_address0 (tarray tdouble n) (SUB delt (Z.of_nat t)) p2)
+  by auto with field_compatible.
+ rewrite <- !(data_at_share_join Ers Ers2 Ews) by auto with shares.
 cancel.
 }
- unfold fclo. rewrite Zlength_map, Zlength_iota. lia. lia.
-
  forward.
 deadvars!.
-freeze FR2 := - (spectasks_list dtask_package (fclo gv numt dtp) inp ANSWER)
+freeze FR2 := - (spectasks_list dtask_package (fclo gv T dtp) inp ANSWER)
    (data_at Ews (tptr t_dtask) dtp (gv _dtasks)).
 unfold spectasks_list.
 unfold fclo at 2.
 rewrite Zlength_map, Zlength_iota by lia.
-forward_for_simple_bound numt
+forward_for_simple_bound T
   (EX t:Z, 
      PROP ()
-     LOCAL (temp _result (Vfloat (partial_dotprod_f t numt (v1, v2)));
-     temp _T (vint numt); gvars gv)
+     LOCAL (temp _result (Vfloat (partial_dotprod_f t T (v1, v2)));
+     temp _T (vint T); gvars gv)
      SEP (FRZL FR2;
      data_at Ews (tptr t_dtask) dtp (gv _dtasks);
      pred_sepcon
-      (ith_spectask dtask_package (fclo gv numt dtp) inp ANSWER)
-      (fun i : Z => 0 <= i < numt)))%assert.
+      (ith_spectask dtask_package (fclo gv T dtp) inp ANSWER)
+      (fun i : Z => 0 <= i < T)))%assert.
 +
 entailer!.
 +
@@ -908,9 +787,9 @@ forward.
 rewrite <- field_at_SUB_t_DOT_result by (auto; lia).
 forward.
 forward.
- pose proof (delta_range (Zlength v1) numt) ltac:(lia) ltac:(lia) t ltac:(lia).
- pose proof (delta_range (Zlength v1) numt) ltac:(lia) ltac:(lia) (t+1) ltac:(lia).
- pose proof (delta_S (Zlength v1) ltac:(lia) numt t ltac:(lia)).
+ pose proof (delta_range (Zlength v1) T) ltac:(lia) ltac:(lia) t ltac:(lia).
+ pose proof (delta_range (Zlength v1) T) ltac:(lia) ltac:(lia) (t+1) ltac:(lia).
+ pose proof (delta_S (Zlength v1) ltac:(lia) T t ltac:(lia)).
  fold n in H11, H12, H13.
  fold delt in H11,H12,H13.
 entailer!.
@@ -919,8 +798,7 @@ entailer!.
          H17 H16 H15 H14.
  f_equal.
  unfold partial_dotprod_f, dotprod_f.
- rewrite !Zlength_map.
- rewrite !Zlength_combine.
+ rewrite !Zlength_map, !Zlength_combine.
  rewrite <- H.
  rewrite !Z.min_id.
  rewrite iota_S by lia.
@@ -939,29 +817,22 @@ entailer!.
  fold delt.
  auto.
 *
-rewrite (pred_sepcon_isolate t zeq _ (fun i : Z => 0 <= i < numt)) by lia.
+rewrite (pred_sepcon_isolate t zeq _ (fun i : Z => 0 <= i < T)) by lia.
 unfold ith_spectask.
 rewrite Zlength_map. 
 rewrite !Znth_map by (rewrite Zlength_iota; lia).
 rewrite !sepcon_assoc.
 apply sepcon_derives.
 apply derives_refl.
-replace (fst (Znth t (fclo gv numt dtp))) with (gv _dotprod_worker).
-2:{ unfold fclo.
-  rewrite Znth_map by (rewrite Zlength_iota; lia).
-  reflexivity.
-}
+replace (fst (Znth t (fclo gv T dtp))) with (gv _dotprod_worker)
+  by (unfold fclo; list_solve).
 apply sepcon_derives.
 apply derives_refl.
 change task_pred with dtask_pred.
 unfold dtask_pred.
 simpl.
-rewrite prop_true_andp.
-2:{
-rewrite Znth_iota by lia.
-rewrite !Zlength_sublist by lia.
-split; lia.
-}
+rewrite prop_true_andp
+ by (rewrite Znth_iota by lia; rewrite !Zlength_sublist; lia).
 rewrite !Znth_iota by lia.
 rewrite !Zlength_sublist by lia.
 unfold fclo.
