verif_parsplit.v
@@ -15,7 +15,7 @@ Section TASK.
  Variable TP : task_package.
 
 Lemma task_inv_exclusive:
- forall numt b p, exclusive_mpred (task_inv TP numt b p).
+ forall T b p, exclusive_mpred (task_inv TP T b p).
 Proof.
 intros.
 unfold task_inv.
@@ -33,13 +33,13 @@ Qed.
 Lemma body_thread_worker: semax_body Vprog (Gprog TP) f_thread_worker (thread_worker_spec TP).
 Proof.
 start_function.
-set (numt := fst numt_gv).
-set (gv := snd numt_gv).
-clearbody numt. clearbody gv. clear numt_gv.
+set (T := fst T_gv).
+set (gv := snd T_gv).
+clearbody T. clearbody gv. clear T_gv.
 unfold bind_ret in POSTCONDITION.  (* bug? *)
 forward.
 forward_loop (PROP ( )  LOCAL (temp _t arg; temp _arg arg)  
-                      SEP (task_locks TP numt arg)).
+                      SEP (task_locks TP T arg)).
 entailer!.
 unfold task_locks.
 Intros go done.
@@ -48,14 +48,14 @@ assert (Ers <> Share.bot). {
   pose proof readable_Ers. intro; rewrite H0 in H.
   apply unreadable_bot; auto.
 }
-forward_call (Ers,go,task_inv TP numt ASK arg).
+forward_call (Ers,go,task_inv TP T ASK arg).
 unfold task_inv at 2.
 Intros f clo contents.
 forward.
 forward.
-forward_call (numt, clo, contents).
+forward_call (T, clo, contents).
 forward.
-forward_call release_simple (Ers, done, task_inv TP numt ANSWER arg).
+forward_call release_simple (Ers, done, task_inv TP T ANSWER arg).
 lock_props.
 apply task_inv_exclusive.
 unfold task_inv.
@@ -67,12 +67,12 @@ entailer!.
 Qed.
 
 Lemma bundle_task_locks:
- forall numt go done p,
+ forall T go done p,
    field_at Ers t_task (DOT _go) (ptr_of go) p
   * field_at Ers t_task (DOT _done) (ptr_of done) p
-  * lock_inv Ers go (task_inv TP numt ASK p)
-  * lock_inv Ers done (task_inv TP numt ANSWER p)
-  |-- task_locks TP numt p.
+  * lock_inv Ers go (task_inv TP T ASK p)
+  * lock_inv Ers done (task_inv TP T ANSWER p)
+  |-- task_locks TP T p.
 Proof.
 intros.
 unfold task_locks.
@@ -81,10 +81,10 @@ cancel.
 Qed.
 
 Lemma bundle_ith_task:
- forall (i: Z) (p: val) (n: Z) (fclo: list (val*val)) (go done: lock_handle) 
+ forall (i: Z) (p: val) (T: Z) (fclo: list (val*val)) (go done: lock_handle) 
    go' done' f clo,
- let pi := field_address (tarray t_task n) (SUB i) p in 
-  n = Zlength fclo ->
+ let pi := field_address (tarray t_task T) (SUB i) p in 
+  T = Zlength fclo ->
   JMeq f (fst (Znth i fclo)) ->
   JMeq clo (snd (Znth i fclo)) ->
   JMeq go' (ptr_of go) ->
@@ -93,17 +93,16 @@ Lemma bundle_ith_task:
   * field_at Ers2 t_task (DOT _done) done' pi
   * field_at Ews t_task (DOT _f) f pi
   * field_at Ews t_task (DOT _closure) clo pi
-  * lock_inv comp_Ers go (task_inv TP n ASK pi)
-  * lock_inv comp_Ers done (task_inv TP n ANSWER pi)
+  * lock_inv comp_Ers go (task_inv TP T ASK pi)
+  * lock_inv comp_Ers done (task_inv TP T ANSWER pi)
  |-- ith_task TP fclo p i.
 Proof.
 intros.
-unfold ith_task.
+unfold ith_task. Exists go done.
 apply JMeq_eq in H0, H1, H2, H3.
 subst.
-Exists go done.
-rewrite !field_at_data_at.
 subst pi.
+rewrite !field_at_data_at.
 repeat change ([?a; ?b]) with ([a]++[b]).
 rewrite !field_address_app.
 simpl.
@@ -114,7 +113,7 @@ Lemma body_make_tasks: semax_body Vprog (Gprog TP)
                            f_make_tasks (make_tasks_spec TP).
 Proof.
 start_function.
-forward_call (tarray t_task n, gv). {
+forward_call (tarray t_task T, gv). {
   apply prop_right.
   simpl.
   normalize. do 3 f_equal. lia.
@@ -129,27 +128,22 @@ forward.
 entailer!.
 Intros.
 rewrite data_at__tarray.
-freeze FR0 := - (mem_mgr gv) (data_at _ (tarray t_task n) _ _).
+freeze FR0 := - (mem_mgr gv) (data_at _ (tarray t_task T) _ _).
 clear H0.
-assert_PROP (field_compatible (tarray t_task n) [] p). entailer!.
+assert_PROP (field_compatible (tarray t_task T) [] p). entailer!.
 pose (lock_bindings := fun go_done => (ptr_of (fst go_done),(ptr_of (snd go_done), 
                          (Vundef,Vundef)))).
-forward_for_simple_bound n (EX i:Z, 
-   PROP() LOCAL (temp _tasks p; gvars gv; temp _n (vint n))
+forward_for_simple_bound T (EX i:Z, 
+   PROP() LOCAL (temp _tasks p; gvars gv; temp _T (vint T))
    SEP (FRZL FR0; mem_mgr gv;
        data_at_ Ews (tarray t_task 1) p;
-       pred_sepcon (ith_task TP (Zrepeat (Vundef,Vundef) n) p) (fun j => 1 <= j < i);
-       data_at_ Ews (tarray t_task (n-i)) (field_address0 (tarray t_task n) (SUB i) p)))%assert.
+       pred_sepcon (ith_task TP (Zrepeat (Vundef,Vundef) T) p) (fun j => 1 <= j < i);
+       data_at_ Ews (tarray t_task (T-i)) (field_address0 (tarray t_task T) (SUB i) p)))%assert.
 -
 entailer!.
-replace  (fun j : Z => 1 <= j < 1) with (fun _ : Z => False)
-  by (extensionality j; apply prop_ext; intuition lia).
-rewrite !pred_sepcon_False.
-cancel.
-pattern n at 2.
-replace n with (1 + (n-1)) by lia.
-rewrite <- !Zrepeat_app by lia.
-rewrite split2_data_at_Tarray_app with (mid:=1) by Zlength_solve.
+sep_apply data_at_data_at_.
+rewrite !pred_sepcon_False' by lia.
+rewrite split2_data_at__Tarray_app with (mid:=1) by lia.
 cancel.
 -
 set (U := data_at_ Ews (tarray t_task 1) p).
@@ -158,32 +152,26 @@ assert_PROP
   (force_val
         (sem_binary_operation' Oadd (tptr (Tstruct _task noattr)) tuint
            p (vint i))
-  =  field_address0 (tarray t_task n) (SUB i) p). {
+  =  field_address0 (tarray t_task T) (SUB i) p). {
   entailer!.
   rewrite field_address0_offset by auto with field_compatible.
   simpl; f_equal; lia.
 }
 rewrite H2; clear H2.
-rewrite data_at__eq.
-change (default_val _) with (Zrepeat (Vundef, (Vundef, (Vundef, Vundef))) (n - i)).
-pattern (n-i) at 2.
-replace (n-i) with (1 + (n-(i+1))) by lia.
-rewrite <- Zrepeat_app by lia.
-pose proof (split2_data_at_Tarray_app 1 (n-i)).
-rewrite H2 by list_solve. clear H2.
-erewrite data_at_singleton_array_eq by reflexivity.
+rewrite (split2_data_at__Tarray_app 1 (T-i)) by list_solve.
 Intros.
+rewrite data__at_singleton_array_eq.
 forward_call (gv, fun _ : lock_handle => 
-                           task_inv TP n ASK (field_address (tarray t_task n) (SUB i) p)).
+                           task_inv TP T ASK (field_address (tarray t_task T) (SUB i) p)).
 Intros go.
 forward.
 forward_call (gv, fun _ : lock_handle => 
-                           task_inv TP n ANSWER (field_address (tarray t_task n) (SUB i) p)).
+                           task_inv TP T ANSWER (field_address (tarray t_task T) (SUB i) p)).
 Intros done.
 forward.
-replace  (field_address0 (tarray t_task (n - i)) (SUB 1)
-        (field_address0 (tarray t_task n) (SUB i) p))
-  with  (field_address0 (tarray t_task n) (SUB (i+1)) p).
+replace  (field_address0 (tarray t_task (T - i)) (SUB 1)
+        (field_address0 (tarray t_task T) (SUB i) p))
+  with  (field_address0 (tarray t_task T) (SUB (i+1)) p).
 2: {
  clear - H H0 H1.
  pose proof H0.
@@ -193,16 +181,9 @@ replace  (field_address0 (tarray t_task (n - i)) (SUB 1)
  simpl. normalize. f_equal. lia.
 }
 unfold_data_at (data_at _ t_task _ _).
-
-replace (field_address0 (tarray t_task n) (SUB i) p)
-  with (field_address (tarray t_task n) (SUB i) p).
-2:{
-rewrite field_address_offset by auto with field_compatible.
-rewrite field_address0_offset by auto with field_compatible.
-reflexivity.
-}
-set (pi :=  field_address (tarray t_task n) (SUB i) p).
-
+replace (field_address0 (tarray t_task T) (SUB i) p)
+  with (field_address (tarray t_task T) (SUB i) p)
+ by auto with field_compatible.
 rewrite <- !(lock_inv_share_join Ers comp_Ers Tsh)
   by (auto with shares).
 rewrite <- (field_at_share_join Ers Ers2 Ews t_task (DOT _go))
@@ -211,19 +192,15 @@ rewrite <- (field_at_share_join Ers Ers2 Ews t_task (DOT _done))
   by (auto with shares).
 
 Intros.
-sep_apply (bundle_task_locks n go done pi).
-
-pose proof (bundle_ith_task i p n 
-   (Zrepeat (Vundef,Vundef) n) go done (ptr_of go) (ptr_of done)
+sep_apply (bundle_task_locks T go done).
+sep_apply (bundle_ith_task i p T 
+   (Zrepeat (Vundef,Vundef) T) go done (ptr_of go) (ptr_of done)
        Vundef Vundef
       ltac:(list_solve)
       ltac:(apply eq_JMeq; list_solve)
       ltac:(apply eq_JMeq; list_solve)
       (JMeq_refl _)
       (JMeq_refl _)).
-fold pi in H2.
-sep_apply H2. clear H2.
-unfold pi.
 
 (* ISSUE REPORT:
   1. forward_spawn needs to give a lot more error diagnostics 
@@ -232,44 +209,26 @@ unfold pi.
 *)
 
 forward_spawn _thread_worker
-  (field_address (tarray t_task n) (SUB i) p)
-  (n, gv).
-
+  (field_address (tarray t_task T) (SUB i) p)
+  (T, gv).
+  entailer!.
+  apply isptr_is_pointer_or_null; apply field_address_isptr; auto with field_compatible.
 +
-rewrite prop_true_andp by auto.
-cancel.
-+
-red. simpl.
-apply isptr_is_pointer_or_null.
-apply field_address_isptr. auto with field_compatible.
-+
-replace (n - i - 1) with (n - (i+1)) by lia.
+replace (T - i - 1) with (T - (i+1)) by lia.
 entailer!.
-rewrite !pred_sepcon_eq.
-Intros al.
-Exists (i::al).
-entailer!.
-split.
-intro. 
-split; intro. destruct H10. subst; lia. rewrite H8 in H10. lia.
-destruct (zeq x i). subst. left; auto. right. rewrite H8. lia.
-constructor; auto. intro. rewrite H8 in H10. lia.
-simpl iter_sepcon.
-unfold U.
+rewrite (pred_sepcon_isolate i zeq _ (fun j : Z => 1 <= j < i + 1)) by lia.
+subst U.
 cancel.
+apply derives_refl'; f_equal. extensionality j; apply prop_ext; lia.
 - (* after the loop *)
 forward.
 Exists p.
 thaw FR0.
 unfold task_array.
-rewrite Zlength_Zrepeat.
-entailer!.
-rewrite data_at__eq.
+rewrite Zlength_Zrepeat by lia.
 rewrite Znth_Zrepeat by lia.
-change (default_val (tarray t_task 1))
- with  [(Vundef, (Vundef, (Vundef, Vundef)))].
-cancel.
-lia.
+change (data_at _ _ _ p) with (data_at_ Ews (tarray t_task 1) p).
+entailer!.
 Qed.
 
 Lemma body_initialize_task: semax_body Vprog (Gprog TP) 
@@ -293,16 +252,13 @@ rewrite Zlength_upd_Znth.
 rewrite upd_Znth_same by lia.
 entailer!.
 apply derives_refl'.
-apply pred_sepcon_strong_proper.
-intros. tauto.
+apply pred_sepcon_strong_proper. tauto.
 intros.
 unfold ith_task.
-apply exp_congr; intro go.
-apply exp_congr; intro done.
 list_simplify.
 -
-set (U := data_at _ _ _ _).
 rewrite (pred_sepcon_isolate i zeq) by lia.
+set (U := data_at _ _ _ _).
 set (V := pred_sepcon _ _).
 Intros.
 unfold ith_task.
@@ -311,22 +267,21 @@ forward.
 forward.
 unfold task_array.
 rewrite (pred_sepcon_isolate i zeq) by list_simplify.
-replace (pred_sepcon _ _) with V.
-unfold U.
 rewrite Zlength_upd_Znth.
+replace (pred_sepcon _ _) with V.
++
+subst U.
 entailer!.
-list_simplify.
-cancel.
 unfold ith_task.
 Exists go done.
 list_simplify.
 cancel.
++
 subst V.
-apply pred_sepcon_strong_proper.
-intros. list_simplify.
-intros.
+apply pred_sepcon_strong_proper; intros.
+list_simplify.
 unfold ith_task.
-destruct H0.
+destruct H1.
 list_simplify.
 Qed.
 
@@ -356,7 +311,7 @@ unfold task_array.
 Intros.
 forward_for_simple_bound (Zlength fclo)
   (EX i:Z, 
-    PROP() LOCAL(temp _tasks p; temp _n (vint (Zlength fclo)))
+    PROP() LOCAL(temp _tasks p; temp _T (vint (Zlength fclo)))
     SEP (data_at Ews (tarray t_task 1) [(Vundef, (Vundef, Znth 0 fclo))] p;
            pred_sepcon (ith_husk fclo inputs p) (fun j : Z => 1 <= j < i);
            pred_sepcon (ith_task TP fclo p) (fun j : Z => i <= j < Zlength fclo);
@@ -368,9 +323,7 @@ entailer!.
 replace (fun y : Z => 0 <= y < Zlength fclo /\ y <> 0)
   with (fun j : Z => 1 <= j < Zlength fclo)
   by (extensionality j; apply prop_ext; split; intro; lia).
-replace (fun j => 1 <= j < 1) with (fun j :Z => False)
-  by (extensionality j; apply prop_ext; split; intro; lia).
-rewrite pred_sepcon_False.
+rewrite (pred_sepcon_False' (fun j : Z => 1 <= j < 1)) by lia.
 cancel.
 -
 rewrite (pred_sepcon_isolate i zeq (ith_spectask TP fclo inputs ASK) ) by lia.
@@ -389,11 +342,7 @@ unfold ith_task at 2.
 Intros go done.
 freeze FR2 := - 
   (field_at Ers2 (tarray t_task (Zlength fclo)) [StructField _go; ArraySubsc i] _ p)
-  (field_at Ews (tarray t_task (Zlength fclo)) [StructField _f; ArraySubsc i] _ p)
-  (field_at Ews (tarray t_task (Zlength fclo)) [StructField _closure; ArraySubsc i] _ p)
-  (func_ptr' (task_f_spec TP) (fst (Znth i fclo)))
-  (lock_inv comp_Ers go _)
-  (task_pred _ (Znth i inputs) ASK (snd (Znth i fclo))).
+  (lock_inv comp_Ers go _).
 forward.
 thaw FR2.
 set (clo := snd (Znth i fclo)).
@@ -411,10 +360,8 @@ assert (
  cancel.
  rewrite !field_at_data_at.
  simpl.
- apply derives_refl'.
- f_equal; f_equal;
- change ([?a; ArraySubsc i]) with ([a]++[ArraySubsc i]);
- rewrite field_address_app; reflexivity.
+ repeat change ([?a; ArraySubsc i]) with ([a]++[ArraySubsc i]).
+ rewrite !field_address_app. apply derives_refl.
 }
 rewrite <- !(field_at_share_join Ers Ers2 Ews) by apply join_Ers_Ers2.
 sep_apply H2. clear H2.
@@ -437,10 +384,7 @@ Exists go done.
 fold clo.
 cancel.
 -
-replace  (fun j : Z => Zlength fclo <= j < Zlength fclo)
-  with (fun j:Z => False) 
- by (clear; extensionality j; apply prop_ext; split; intros; lia).
-rewrite !pred_sepcon_False.
+rewrite !(pred_sepcon_False'  (fun j : Z => Zlength fclo <= j < Zlength fclo)) by lia.
 unfold ith_spectask.
 Intros.
 forward.
@@ -457,7 +401,7 @@ assert (func_ptr' (task_f_spec TP) (fst (Znth 0 fclo))
 sep_apply H1; clear H1.
 forward_for_simple_bound (Zlength fclo)
   (EX i:Z, 
-    PROP() LOCAL(temp _tasks p; temp _n (vint (Zlength fclo)))
+    PROP() LOCAL(temp _tasks p; temp _T (vint (Zlength fclo)))
     SEP (data_at Ews (tarray t_task 1) [(Vundef, (Vundef, Znth 0 fclo))] p;
            pred_sepcon (ith_task TP fclo p) (fun j : Z => 1 <= j < i);
            pred_sepcon (ith_husk fclo inputs p) (fun j : Z => i <= j < Zlength fclo);
@@ -465,10 +409,7 @@ forward_for_simple_bound (Zlength fclo)
                  (fun j : Z => 1 <= j < i);
            ith_spectask TP fclo inputs ANSWER 0))%assert.
 +
-replace  (fun j : Z => 1 <= j < 1)
-  with (fun j:Z => False) 
- by (clear; extensionality j; apply prop_ext; split; intros; lia).
-rewrite !pred_sepcon_False.
+rewrite !(pred_sepcon_False'  (fun j : Z => 1 <= j < 1)) by lia.
 entailer!.
 +
 rewrite (pred_sepcon_isolate i zeq  (ith_husk fclo inputs p) ) by lia.
@@ -503,15 +444,9 @@ sep_apply (data_at_value_eq Ers Ers2
                         (field_address t_task (DOT _f)
          (field_address (tarray t_task (Zlength fclo)) (SUB i) p))); auto.
 Intros; subst f clo.
-sep_apply (data_at_share_join Ers Ers2 Ews (tptr tvoid) 
-                       (snd (Znth i fclo))
-      (field_address t_task (DOT _closure)
-         (field_address (tarray t_task (Zlength fclo)) (SUB i) p))); auto with shares.
-sep_apply (data_at_share_join Ers Ers2 Ews 
-             (tptr (Tfunction (Tcons (tptr tvoid) Tnil) tvoid cc_default))
-                       (fst (Znth i fclo))
-      (field_address t_task (DOT _f)
-         (field_address (tarray t_task (Zlength fclo)) (SUB i) p))); auto with shares.
+
+sep_apply (data_at_share_join Ers Ers2 Ews); auto with shares.
+sep_apply (data_at_share_join Ers Ers2 Ews); auto with shares.
 rewrite <- !sepcon_assoc.
 assert (BIT := bundle_ith_task i p (Zlength fclo) fclo go done
                     (ptr_of go) (ptr_of done) (fst (Znth i fclo)) (snd (Znth i fclo))
@@ -528,17 +463,13 @@ replace (fun y : Z => i <= y < Zlength fclo /\ y <> i)
  by (clear; extensionality j; apply prop_ext; split; intros; lia).
 sep_apply task_pred_contents_eq.
 Intros. subst contents.
-cancel.
 unfold ith_spectask.
 cancel.
 +
 entailer!.
 unfold task_array, spectasks_list.
 rewrite prop_true_andp by auto.
-replace (fun y : Z => Zlength fclo <= y < Zlength fclo)
-  with  (fun j : Z => False)
- by (clear; extensionality j; apply prop_ext; split; intros; lia).
-rewrite pred_sepcon_False.
+rewrite (pred_sepcon_False' (fun y : Z => Zlength fclo <= y < Zlength fclo)) by lia.
 rewrite (pred_sepcon_isolate 0 zeq _ (fun i : Z => 0 <= i < Zlength fclo)) by lia.
 replace  (fun y : Z => 0 <= y < Zlength fclo /\ y <> 0)
   with   (fun y : Z => 1 <= y < Zlength fclo)
